Proved Reflexivity of LR over types

LRInduction.v
@@ -18,7 +18,7 @@ Fixpoint LR_rec0
     (forall {Δ} (h : [ |- Δ]),
       P0(H1.(_F1) h)) ->
     (forall {Δ a} (h1 : [ |- Δ ]) 
-      (h2 : @Rel1Te _ rec0 Δ a (F H0) (_F H0 h1; H1.(_F1) h1)),
+      (h2 : @Rel1Te _ rec0 Δ a (F H0) (LRValidMk (_F H0 h1) (H1.(_F1) h1))),
       P0 (_G1 H1 h1 h2)) ->
     P0 (LRPi rec0 H0 H1)) 
   ->
@@ -33,8 +33,6 @@ Proof.
    intros;
    apply LR_rec0; try assumption.
 Defined.
-
-Check LR_rec0.
 
 (*TODO : get a good induction principle*)
 (*Scheme LR_rect := Induction for LR Sort Type.*)
@@ -53,7 +51,7 @@ Fixpoint LR_rec1
     (forall {Δ} (h : [ |- Δ]),
       P0 (H1.(_F1) h)) ->
     (forall {Δ a} (h1 : [ |- Δ ]) 
-      (h2 : @Rel1Te _ rec0 Δ a (F H0) (_F H0 h1; H1.(_F1) h1)),
+      (h2 : @Rel1Te _ rec0 Δ a (F H0) (LRValidMk (_F H0 h1) (H1.(_F1) h1))),
       P0 (_G1 H1 h1 h2)) ->
     P0 (LRPi rec0 H0 H1)) 
   ->
@@ -69,7 +67,7 @@ Fixpoint LR_rec1
   (forall {Δ} (h : [ |- Δ]),
     P1 (H1.(_F1) h)) ->
   (forall {Δ a} (h1 : [ |- Δ ]) 
-    (h2 : @Rel1Te _ rec1 Δ a (F H0) (_F H0 h1; H1.(_F1) h1)),
+    (h2 : @Rel1Te _ rec1 Δ a (F H0) (LRValidMk (_F H0 h1) (H1.(_F1) h1))),
     P1 (_G1 H1 h1 h2)) ->
   P1 (LRPi rec1 H0 H1)) 
   ->
@@ -78,7 +76,7 @@ Fixpoint LR_rec1
   (forall (Γ : context) (A : term) {l' l_}
     (H : [kit0 | Γ ||- A]),
     
-    P0 (projT2 H) ->
+    P0 H.(valid) ->
     P1 (@LRemb _ _ _ _ l' l_ H)) ->
 
     P1 lr.
@@ -93,10 +91,81 @@ Proof.
   eapply LR_rec1; try eassumption.
   eapply X4.
   destruct H.
-  inversion l.
+  inversion valid.
   1, 4 : inversion l_0.
   all : eapply LR_rec0; assumption.
 Defined.
+
+Definition LR_rect0 : forall
+  (P0 : forall {c t rEq rTe rTeEq} ,
+   @LR zero rec0 c t rEq rTe rTeEq  -> Type),
+  (forall (Γ : context) (A : term) (neA : [Γ ||-ne A]),
+    P0 (LRne rec0 neA))
+  ->
+  (forall (Γ : context) (A : term) (H0 : [ Γ ||-0Π A ]) (H1 : TyPiRel1 (LR rec0) H0),
+    (forall {Δ} (h : [ |- Δ]),
+      P0(H1.(_F1) h)) ->
+    (forall {Δ a} (h1 : [ |- Δ ]) 
+      (h2 : @Rel1Te _ rec0 Δ a (F H0) (LRValidMk (_F H0 h1) (H1.(_F1) h1))),
+      P0 (_G1 H1 h1 h2)) ->
+    P0 (LRPi rec0 H0 H1)) 
+  ->
+   forall(c : context) (t : term) (rEq rTe : term -> Type)
+  (rTeEq  : term -> term -> Type) (lr : LR rec0 c t rEq rTe rTeEq ),
+   P0 lr.
+Proof.
+  intros.
+  eapply LR_rec0; eassumption.
+Defined.
+
+Definition LR_rect1 : 
+  forall 
+  (P0 : forall {c t rEq rTe rTeEq} ,
+   @LR zero rec0 c t rEq rTe rTeEq  -> Type)
+  (P1 : forall {c t rEq rTe rTeEq} ,
+   @LR one rec1 c t rEq rTe rTeEq  -> Type),
+  (forall (Γ : context) (A : term) (neA : [Γ ||-ne A]),
+    P0 (LRne rec0 neA)) 
+  ->
+  (forall (Γ : context) (A : term) (H0 : [ Γ ||-0Π A ]) (H1 : TyPiRel1 (LR rec0) H0),
+    (forall {Δ} (h : [ |- Δ]),
+      P0 (H1.(_F1) h)) ->
+    (forall {Δ a} (h1 : [ |- Δ ]) 
+      (h2 : @Rel1Te _ rec0 Δ a (F H0) (LRValidMk (_F H0 h1) (H1.(_F1) h1))),
+      P0 (_G1 H1 h1 h2)) ->
+    P0 (LRPi rec0 H0 H1)) 
+  ->
+
+
+  (forall (Γ : context) (h : [  |- Γ]) {l' l_},
+    P1 (LRU rec1 h l' l_)) 
+  ->
+  (forall (Γ : context) (A : term) (neA : [Γ ||-ne A]),
+    P1 (LRne rec1 neA)) 
+  ->
+  (forall (Γ : context) (A : term) (H0 : [ Γ ||-0Π A ]) (H1 : TyPiRel1 (LR rec1) H0),
+  (forall {Δ} (h : [ |- Δ]),
+    P1 (H1.(_F1) h)) ->
+  (forall {Δ a} (h1 : [ |- Δ ]) 
+    (h2 : @Rel1Te _ rec1 Δ a (F H0) (LRValidMk (_F H0 h1) (H1.(_F1) h1))),
+    P1 (_G1 H1 h1 h2)) ->
+  P1 (LRPi rec1 H0 H1)) 
+  ->
+
+
+  (forall (Γ : context) (A : term) {l' l_}
+    (H : [kit0 | Γ ||- A]),
+    
+    P0 H.(valid) ->
+    P1 (@LRemb _ _ _ _ l' l_ H)) ->
+  forall (c : context) (t : term) (rEq rTe : term -> Type)
+  (rTeEq  : term -> term -> Type) (lr : LR rec1 c t rEq rTe rTeEq ),
+    P1 lr.
+Proof.
+  intros.
+  eapply LR_rec1; eassumption.
+Defined.
+
 
 
 (*Definition LR_rect : forall 
